src/SemanticsEquivalence.v
@@ -1,0 +1,431 @@
+Add LoadPath "~/JB/minikanren-coq/src/".
+
+Require Import List.
+Import ListNotations.
+Require Import Stream.
+Require Import Unify.
+Require Import MiniKanrenSyntax.
+Require Import OperationalSem.
+Require Import DenotationalSem.
+Require Import Omega.
+
+Definition in_denotational_sem_subst (s : subst) (f : gt_fun) : Prop :=
+  exists (f' : gt_fun), gt_fun_eq (subst_gt_fun_compose s f') f.
+
+Inductive in_denotational_sem_state' : state' -> gt_fun -> Prop :=
+| dsst'Leaf : forall g s n f (Hgoal : in_denotational_sem_goal g f)
+                             (Hsubst : in_denotational_sem_subst s f),
+                             in_denotational_sem_state' (Leaf g s n) f
+| dsst'SumL : forall st1' st2' f (Hst1' : in_denotational_sem_state' st1' f),
+                                 in_denotational_sem_state' (Sum st1' st2') f
+| dsst'SumR : forall st1' st2' f (Hst2' : in_denotational_sem_state' st2' f),
+                                 in_denotational_sem_state' (Sum st1' st2') f
+| dsst'Prod : forall st' g f (Hgoal : in_denotational_sem_goal g f)
+                             (Hst' : in_denotational_sem_state' st' f),
+                             in_denotational_sem_state' (Prod st' g) f.
+
+Hint Constructors in_denotational_sem_state'.
+
+Inductive in_denotational_sem_state : state -> gt_fun -> Prop :=
+| dsstState : forall st' f (Hst' : in_denotational_sem_state' st' f),
+                           in_denotational_sem_state (State st') f.
+
+Hint Constructors in_denotational_sem_state.
+
+Definition in_denotational_analog (t : trace) (f : gt_fun) : Prop :=
+  exists (s : subst) (n : nat), in_stream (Answer s n) t /\ in_denotational_sem_subst s f.
+
+Lemma answer_correct
+      (s : subst)
+      (n : nat)
+      (f : gt_fun)
+      (HInDS : in_denotational_sem_subst s f)
+      (st' : state')
+      (st : state)
+      (EV : eval_step st' (Answer s n) st) :
+      in_denotational_sem_state' st' f.
+Proof.
+  remember (Answer s n) as l.
+  induction EV; good_inversion Heql.
+  2, 3: auto.
+  destruct HInDS as [f' ff'_con].
+  constructor.
+  { constructor. red.
+    specialize (gt_fun_eq_apply _ _ t1 ff'_con). intro. rewrite <- H.
+    specialize (gt_fun_eq_apply _ _ t2 ff'_con). intro. rewrite <- H0.
+    rewrite gt_fun_apply_compose. rewrite gt_fun_apply_compose.
+    rewrite compose_correctness. rewrite compose_correctness.
+    apply unify_unifies in u. rewrite u. reflexivity. }
+  { red. exists (subst_gt_fun_compose s' f').
+    red. intros. red.
+    red in ff'_con. specialize (ff'_con x). red in ff'_con.
+    rewrite <- ff'_con. unfold subst_gt_fun_compose.
+    replace (fun x0 : name => apply_gt_fun f' (apply_subst s' (Var x0)))
+      with (subst_gt_fun_compose s' f').
+    2: reflexivity.
+    rewrite gt_fun_apply_compose. rewrite compose_correctness.
+    reflexivity. }
+Qed.
+
+Lemma next_state_correct
+      (f : gt_fun)
+      (st : state)
+      (HInDS : in_denotational_sem_state st f)
+      (st' : state')
+      (wfState : well_formed_state' st')
+      (h : label)
+      (EV : eval_step st' h st) :
+      in_denotational_sem_state' st' f.
+Proof.
+  induction EV; good_inversion HInDS.
+  { good_inversion Hst'.
+    { good_inversion Hst1'; constructor; auto. }
+    { good_inversion Hst2'; constructor; auto. } }
+  { good_inversion Hst'. good_inversion Hst'0. auto. }
+  { good_inversion wfState. good_inversion Hst'.
+    constructor; auto. econstructor; eauto.
+    intros HIn. apply freshCorrect in HIn. omega. }
+  { good_inversion Hst'. auto. }
+  { auto. }
+  { good_inversion wfState. good_inversion Hst'; auto. }
+  { good_inversion Hst'. constructor; auto.
+    eapply answer_correct; eauto. }
+  { good_inversion wfState. good_inversion Hst'. auto. }
+  { good_inversion wfState. good_inversion Hst'.
+    { good_inversion Hst1'. constructor; auto.
+      eapply answer_correct; eauto. }
+    { good_inversion Hst2'. auto. } }
+Qed.
+
+Lemma search_correctness_generalized
+      (st   : state)
+      (wfSt : well_formed_state st)
+      (f    : gt_fun)
+      (t    : trace)
+      (HOP  : op_sem st t)
+      (HDA  : in_denotational_analog t f) :
+      in_denotational_sem_state st f.
+Proof.
+  revert HOP wfSt. revert st.
+  red in HDA. destruct HDA as [s [n [HInStr HInDS]]].
+  remember (Answer s n) as l. induction HInStr.
+  { intros. inversion HOP; clear HOP; subst.
+    constructor. eapply answer_correct; eauto. }
+  { specialize (IHHInStr Heql). intros.
+    inversion HOP; clear HOP; subst.
+    inversion wfSt; clear wfSt; subst.
+    specialize (well_formedness_preservation _ _ _ EV wfState).
+    intro wf_st0.
+    specialize (IHHInStr st0 OP wf_st0).
+    constructor. eapply next_state_correct; eauto. }
+Qed.
+
+Fixpoint first_nats (k : nat) : list nat :=
+  match k with
+  | 0   => []
+  | S n => n :: first_nats n
+  end.
+
+Lemma first_nats_less (n k : nat) (H : In n (first_nats k)) : n < k.
+Proof.
+  induction k.
+  { inversion H. }
+  { inversion H. { omega. } { apply IHk in H0. omega. } }
+Qed.
+
+Lemma search_correctness
+      (g   : goal)
+      (k   : nat)
+      (HC  : closed_goal_in_context (first_nats k) g)
+      (f   : gt_fun)
+      (t   : trace)
+      (HOP : op_sem (State (Leaf g empty_subst k)) t)
+      (HDA : in_denotational_analog t f) : in_denotational_sem_goal g f.
+Proof.
+  remember (State (Leaf g empty_subst k)) as st.
+  assert (in_denotational_sem_state st f).
+  { eapply search_correctness_generalized; eauto.
+    subst. constructor. constructor.
+    intros. apply HC in H. apply first_nats_less. auto. }
+  subst. inversion H. inversion Hst'. auto.
+Qed.
+
+Lemma unfier_from_gt_unifier
+      (t1 t2 : term)
+      (f : gt_fun)
+      (f_unifies : gt_eq (apply_gt_fun f t1) (apply_gt_fun f t2)) :
+      exists s, unifier s t1 t2 /\ in_denotational_sem_subst s f.
+Proof. admit. Admitted.
+
+Lemma gt_fun_eq_trans
+      (f1 f2 f3 : gt_fun)
+      (eq12 : gt_fun_eq f1 f2)
+      (eq23 : gt_fun_eq f2 f3) :
+      gt_fun_eq f1 f3.
+Proof. admit. Admitted.
+
+Lemma gt_fun_eq_compose
+      (f1 f2 : gt_fun)
+      (eq : gt_fun_eq f1 f2)
+      (s : subst) :
+      gt_fun_eq (subst_gt_fun_compose s f1) (subst_gt_fun_compose s f2).
+Proof. admit. Admitted.
+
+Lemma gt_fun_compose_eq
+      (f : gt_fun)
+      (s1 s2 : subst)
+      (eq : forall t, apply_subst s1 t = apply_subst s2 t) :
+      gt_fun_eq (subst_gt_fun_compose s1 f) (subst_gt_fun_compose s2 f).
+Proof. admit. Admitted.
+
+Lemma subst_gt_fun_compose_assoc_subst
+      (f : gt_fun)
+      (s s' : subst) :
+      gt_fun_eq (subst_gt_fun_compose (compose s s') f)
+                (subst_gt_fun_compose s (subst_gt_fun_compose s' f)).
+Proof. admit. Admitted.
+
+Lemma counter_in_answer
+      (g : goal)
+      (s sr : subst)
+      (n nr : nat)
+      (tr : trace)
+      (OP : op_sem (State (Leaf g s n)) tr)
+      (HIn : in_stream (Answer sr nr) tr) :
+      n <= nr.
+Proof. admit. Admitted.
+
+Lemma prod_op_sem_in
+      (st' : state')
+      (g : goal)
+      (s : subst)
+      (n : nat)
+      (t1 t2 t : trace)
+      (r : label)
+      (OP : op_sem (State (Prod st' g)) t)
+      (OP1 : op_sem (State st') t1)
+      (OP2 : op_sem (State (Leaf g s n)) t2)
+      (HIn1 : in_stream (Answer s n) t1)
+      (HIn2 : in_stream r t2) :
+      in_stream r t.
+Proof. admit. Admitted.
+
+Lemma apply_gt_fun_fv
+      (f1 f2 : gt_fun)
+      (t : term)
+      (f_fv_eq : forall x, (In x (fv_term t)) -> f1 x = f2 x) :
+      gt_eq (apply_gt_fun f1 t) (apply_gt_fun f2 t).
+Proof. admit. Admitted.
+
+Lemma well_formed_subst_in_state_dom
+      (g : goal)
+      (s : subst)
+      (n : nat)
+      (wfSt' : well_formed_state' (Leaf g s n))
+      (x : name)
+      (n_le_x : n <= x) :
+      image s x = None.
+Proof. admit. Admitted.
+
+Lemma well_formed_subst_in_state_vran
+      (g : goal)
+      (s : subst)
+      (n : nat)
+      (wfSt' : well_formed_state' (Leaf g s n))
+      (x : name)
+      (t : term)
+      (img_x : image s x = Some t)
+      (v : name)
+      (v_in : In v (fv_term t)) :
+      v < n.
+Proof. admit. Admitted.
+
+Lemma den_sem_fv_only
+      (f f' : gt_fun)
+      (g : goal)
+      (l : nat)
+      (ff'_eq : forall x, is_fv_of_goal x g -> gt_eq (f x) (f' x))
+      (Hgoal : in_denotational_sem_lev_goal l g f) :
+      in_denotational_sem_lev_goal l g f'.
+Proof. admit. Admitted.
+
+Lemma den_sem_another_fresh_var
+      (b : name -> goal)
+      (s : subst)
+      (n : nat)
+      (wfSt' : well_formed_state' (Leaf (Fresh b) s n))
+      (a1 a2 : name)
+      (a1_fresh : ~ is_fv_of_goal a1 (Fresh b))
+      (a2_fresh : ~ is_fv_of_goal a2 (Fresh b))
+      (fa1 fa2 : gt_fun)
+      (l : nat)
+      (Hgoal_f1 : in_denotational_sem_lev_goal l (b a1) fa1)
+      (f_switch : fa2 a2 = fa1 a1)
+      (f12_eq : forall x, x <> a1 -> x <> a2 -> fa1 x = fa2 x) :
+      in_denotational_sem_lev_goal l (b a2) fa2.
+Proof. admit. Admitted.
+
+Lemma search_completeness_generalized
+      (l     : nat)
+      (g     : goal)
+      (s     : subst)
+      (n     : nat)
+      (wfSt' : well_formed_state' (Leaf g s n))
+      (t     : trace)
+      (HOP   : op_sem (State (Leaf g s n)) t)
+      (f     : gt_fun)
+      (Hgoal : in_denotational_sem_lev_goal l g f)
+      (Hsubst : in_denotational_sem_subst s f) :
+      exists (f' : gt_fun), (in_denotational_analog t f') /\
+                            forall (x : name), x < n -> gt_eq (f x) (f' x).
+Proof.
+  revert HOP. revert t. revert Hgoal Hsubst wfSt'. revert g f s n. induction l.
+  { intros. apply in_denotational_sem_zero_lev in Hgoal. contradiction. }
+  { induction g; intros.
+    { good_inversion Hgoal. }
+    { exists f. split.
+      2: intros; red; auto.
+      good_inversion Hgoal. red in Hsubst. destruct Hsubst as [fs s_fs_f].
+      assert (gt_eq (apply_gt_fun fs (apply_subst s t)) (apply_gt_fun fs (apply_subst s t0))).
+      { red. rewrite <- gt_fun_apply_compose. rewrite <- gt_fun_apply_compose.
+        apply eq_trans with (proj1_sig (apply_gt_fun f t)).
+        { apply gt_fun_eq_apply. auto. }
+        { apply eq_trans with (proj1_sig (apply_gt_fun f t0)); auto.
+          symmetry. apply gt_fun_eq_apply. auto. } }
+      apply unfier_from_gt_unifier in H. destruct H as [u [u_uni u_fs]].
+      good_inversion HOP. good_inversion EV.
+      { specialize (unify_non_unifiable _ _ H5 u u_uni). contradiction. }
+      { rename s' into m. red. exists (compose s m). exists n. split; try constructor.
+        specialize (unify_most_general _ _ _ H5 u u_uni). intro Hmg.
+        red in Hmg. destruct Hmg as [ds u_ds_m]. red in u_fs.
+        destruct u_fs as [fss u_fss_fs]. red. exists (subst_gt_fun_compose ds fss).
+        eapply gt_fun_eq_trans. 2: eauto.
+        eapply gt_fun_eq_trans. eapply subst_gt_fun_compose_assoc_subst.
+        eapply gt_fun_eq_trans. 2: eapply gt_fun_eq_compose; eauto.
+        apply gt_fun_eq_compose.
+        eapply gt_fun_eq_trans. red; symmetry; eapply subst_gt_fun_compose_assoc_subst.
+        apply gt_fun_compose_eq. intros. rewrite u_ds_m. apply compose_correctness. } }
+    { good_inversion HOP. inversion EV; subst.
+      apply well_formedness_preservation in EV; auto. good_inversion EV.
+      good_inversion wfState.
+      specialize (op_sem_exists (State (Leaf g1 s n))). intro p1. destruct p1 as [t1 OP1].
+      specialize (op_sem_exists (State (Leaf g2 s n))). intro p2. destruct p2 as [t2 OP2].
+      specialize (sum_op_sem _ _ _ _ _ OP1 OP2 OP). intro Hinter.
+      good_inversion Hgoal.
+      { specialize (IHg1 f s n Hg Hsubst wfst'1 t1 OP1).
+        destruct IHg1 as [f' [HinDA ff'_eq]]. exists f'. split; auto.
+        red in HinDA. destruct HinDA as [sr [nr [Hin Hsubstr]]].
+        red. exists sr. exists nr. split; auto. constructor.
+        apply (interleave_in _ _ _ Hinter (Answer sr nr)). auto. }
+      { specialize (IHg2 f s n Hg Hsubst wfst'2 t2 OP2).
+        destruct IHg2 as [f' [HinDA ff'_eq]]. exists f'. split; auto.
+        red in HinDA. destruct HinDA as [sr [nr [Hin Hsubstr]]].
+        red. exists sr. exists nr. split; auto. constructor.
+        apply (interleave_in _ _ _ Hinter (Answer sr nr)). auto. } }
+    { good_inversion Hgoal. good_inversion HOP. inversion EV; subst.
+      specialize (op_sem_exists (State (Leaf g1 s n))). intro p1. destruct p1 as [t1 OP1].
+      assert (wfst'1 : well_formed_state' (Leaf g1 s n)).
+      { constructor. good_inversion wfSt'. auto. }
+      specialize (IHg1 f s n Hg1 Hsubst wfst'1 t1 OP1).
+      destruct IHg1 as [f' [HinDA ff'_eq]]. red in HinDA.
+      destruct HinDA as [s' [n' [Hinstr' HDAS']]].
+      specialize (op_sem_exists (State (Leaf g2 s' n'))). intro p2. destruct p2 as [t2 OP2].
+      specialize (counter_in_answer _ _ _ _ _ _ OP1 Hinstr'). intro n_le_n'.
+      assert (wfst'2 : well_formed_state' (Leaf g2 s' n')).
+      { constructor. good_inversion wfSt'. intros.
+        apply lt_le_trans with n; auto. }
+      assert (Hg2' : in_denotational_sem_lev_goal (S l) g2 f').
+      { apply den_sem_fv_only with f; auto. intros. apply ff'_eq.
+        good_inversion wfSt'. auto. }
+      specialize (IHg2 f' s' n' Hg2' HDAS' wfst'2 t2 OP2).
+      destruct IHg2 as [f'' [HinDA f'f''_eq]]. red in HinDA.
+      destruct HinDA as [s'' [n'' [Hinstr'' HDAS'']]].
+      exists f''. split.
+      { red. exists s''. exists n''. split; auto.
+        constructor. eapply prod_op_sem_in; eauto. }
+      { intros. red. apply eq_trans with (proj1_sig (f' x)).
+        { apply ff'_eq. auto. }
+        { apply f'f''_eq. omega. } } }
+    { good_inversion Hgoal. good_inversion HOP. inversion EV; subst.
+      apply well_formedness_preservation in EV; auto. good_inversion EV.
+      rename fn into fa.
+      red in Hsubst. destruct Hsubst as [fs fssf'_eq].
+      remember (fun x => if name_eq_dec x n
+                         then fa a
+                         else fs x) as fs'.
+      remember (fun x => if name_eq_dec x n
+                         then fa a
+                         else if name_eq_dec x a
+                              then (subst_gt_fun_compose s fs') a
+                              else fa x) as fn.
+      assert (H_n_is_fresh : forall x, In n (fv_term (apply_subst s (Var x))) -> x = n).
+      { intros. simpl in H0.
+        destruct (image s x) eqn:eq.
+        { specialize (well_formed_subst_in_state_vran _ _ _ wfSt' _ _ eq _ H0).
+          omega. }
+        { simpl in H0. destruct H0; try contradiction. auto. } }
+      assert (Hgn : in_denotational_sem_lev_goal (S l) (g n) fn).
+      { rewrite Heqfn. apply den_sem_another_fresh_var with s n a fa; auto.
+        { good_inversion wfSt'. intro C. apply freshCorrect in C. omega. }
+        { destruct (name_eq_dec n n); try contradiction. auto. }
+        { intros. destruct (name_eq_dec x n); try contradiction.
+          destruct (name_eq_dec x a); try contradiction. auto. } }
+      assert (Hsubstn: in_denotational_sem_subst s fn).
+      { red. exists fs'. red. intros. red. unfold subst_gt_fun_compose.
+        rewrite Heqfs'. rewrite Heqfn. destruct (name_eq_dec x n).
+        { assert (H_n_is_fresh_2 : apply_subst s (Var n) = Var n).
+          { specialize (well_formed_subst_in_state_dom _ _ _ wfSt' n (le_refl n)).
+            intro. simpl. rewrite H0. auto. }
+          rewrite e. rewrite H_n_is_fresh_2. simpl.
+          destruct (name_eq_dec n n); try contradiction. auto. }
+        { destruct (name_eq_dec x a).
+          { rewrite e. rewrite Heqfs'. auto. }
+          { specialize (Hease x n1). rewrite Hease.
+            red in fssf'_eq. specialize (fssf'_eq x). red in fssf'_eq.
+            rewrite <- fssf'_eq. unfold subst_gt_fun_compose.
+            apply apply_gt_fun_fv. intros. destruct (name_eq_dec x0 n); auto.
+            rewrite e in H0. apply H_n_is_fresh in H0. contradiction. } } }
+      specialize (H n fn s (S n) Hgn Hsubstn wfState t0 OP).
+      destruct H as [f' [HinDA ff'_eq]]. exists f'. split.
+      { red. red in HinDA. destruct HinDA as [s' [n' [Hinstr HDAS]]].
+        exists s'. exists n'. split; auto. constructor; auto. }
+      { intros. assert (x < S n). { omega. }
+        specialize (ff'_eq x H0). red in ff'_eq. red. rewrite <- ff'_eq.
+        rewrite Heqfn. destruct (name_eq_dec x n); try omega.
+        destruct (name_eq_dec x a).
+        { rewrite e.
+          red in fssf'_eq. specialize (fssf'_eq a). red in fssf'_eq.
+          rewrite <- fssf'_eq. unfold subst_gt_fun_compose.
+          apply apply_gt_fun_fv. intros. rewrite Heqfs'.
+          destruct (name_eq_dec x0 n); auto. rewrite e0 in H1.
+          apply H_n_is_fresh in H1. subst. contradiction. }
+        { specialize (Hease x n1). rewrite Hease. auto. } } }
+    { good_inversion Hgoal. good_inversion HOP. inversion EV; subst.
+      apply well_formedness_preservation in EV; auto. good_inversion EV.
+      specialize (IHl (proj1_sig (MiniKanrenSyntax.P n) t) f s n0 Hbody Hsubst wfState t1 OP).
+      destruct IHl as [f' [HinDA ff'_eq]]. exists f'. split; auto.
+      red. red in HinDA. destruct HinDA as [s' [n' [Hinstr HDAS]]].
+      exists s'. exists n'. split; auto. constructor; auto. } }
+Qed.
+
+Lemma search_completeness
+      (g   : goal)
+      (k   : nat)
+      (HC  : closed_goal_in_context (first_nats k) g)
+      (f   : gt_fun)
+      (t   : trace)
+      (HOP : op_sem (State (Leaf g empty_subst k)) t)
+      (HDS : in_denotational_sem_goal g f) :
+      exists (f' : gt_fun), (in_denotational_analog t f') /\
+                            forall (x : name), In x (first_nats k) -> gt_eq (f x) (f' x).
+Proof.
+  apply in_denotational_sem_some_lev in HDS. destruct HDS as [l HDS].
+  assert (wfSt' : well_formed_state' (Leaf g empty_subst k)).
+  { constructor. red in HC. intros. apply first_nats_less; auto. }
+  assert (Hsubst : in_denotational_sem_subst empty_subst f).
+  { red. exists f. red. intros.
+    unfold subst_gt_fun_compose. rewrite apply_empty. reflexivity. }
+  specialize (search_completeness_generalized l g empty_subst k wfSt' t HOP f HDS Hsubst).
+  intro. destruct H as [f' [HinDA ff'eq]]. exists f'. split; auto.
+  intros. apply ff'eq. apply first_nats_less; auto.
+Qed.
